link, sem and psem use option monad

Common/Rc.v
@@ -1,6 +1,7 @@
 Require Import Smallstep.
 Require Import Behavior.
 Require Import Coq.Lists.List.
+Require Import Coq.Program.Basics.
 
 (* 
    Full proof of robust compilation relying on 
@@ -16,11 +17,36 @@ Require Import Coq.Lists.List.
 (* Component id *)
 Variable id : Type.
 Definition interface := list id.
-(* complete program has a complete interface *)
-Variable icomplete : interface -> Prop.
-Definition icomplete2 (i1 i2:interface) := icomplete (i1++i2).
+(* check if the last event of a behavior belongs to an agent,
+   represented by the interface of its components *)
 Variable turn : program_behavior -> interface -> Prop.
+(* check if an interface is complete *)
+Variable icomplete : interface -> Prop.
+(* check if the union of two interfaces is complete *)
+Definition icomplete2 (i1 i2:interface) := icomplete (i1++i2).
+(* Hypothesis unique_interfaces : *)
+(*   forall (i1 i2 i3:interface), *)
+(*     icomplete2 i1 i3 -> icomplete2 i2 i3 -> i1=i2. *)
 
+
+Definition map {A B} (f: A -> B) (o: option A) : option B :=
+  match o with
+  | Some a => Some (f a)
+  | None => None
+  end.
+
+Definition map_compose :
+  forall {A B C} (f1: A -> B) (f2: B -> C) (x:option A),
+    map f2 (map f1 x) = map (compose f2 f1) x.
+Proof.
+  destruct x; auto.
+Qed.
+
+Definition behaves (o: option semantics) b :=
+    match o with
+    | Some p => program_behaves p b
+    | None => False
+    end.
 
 (* 
    The languages.
@@ -29,22 +55,27 @@ Variable turn : program_behavior -> interface -> Prop.
 (* Signature of basic things expected in a language *)
 Module Type Lang.
   (* Type of programs, complete or partial *)
-  Parameter program : Type.
-
-  Parameter get_interface: program -> interface.
-
+  Variable program : Type.
+  Variable get_interface: program -> interface.
   (* checks if a program has a complete interface *)
-  Parameter complete: program -> Prop.
+  Variable complete: program -> Prop.
   (* checks if two programs linked together form a complete program *)
-  Parameter complete2: program -> program -> Prop.
+  Variable complete2: program -> program -> Prop.
 
   (* complete semantics: takes a complete program *)
-  Parameter sem: program -> semantics.
+  Variable sem: option program -> option semantics.
+  (* Variable sem_complete: *)
+  (*   forall (p:program), *)
+  (*     complete p -> exists s, sem (Some p) = Some s. *)
 
   (* partial semantics: takes a program and a matching interface.
      The interface of the program together with the matching interface
      is complete. *)
-  Parameter psem: program -> interface -> semantics.
+  Variable psem: option program -> interface -> option semantics.
+  (* Variable psem_complete: *)
+  (*   forall psi (p:program), *)
+  (*     icomplete2 psi (get_interface p) -> exists s, psem (Some p) psi = Some s. *)
+  (* Variable idefinability: forall (i:interface), exists (p:program), get_interface p = i. *)
 End Lang.
 
 (* Every language is a subtype of Lang and implements its signature *)
@@ -56,8 +87,8 @@ Module T <: Lang.
   Variable get_interface: program -> interface.
   Definition complete (p:program) := icomplete (get_interface p).
   Definition complete2 (p1 p2:program) := icomplete2 (get_interface p1) (get_interface p2).
-  Variable sem: program -> semantics.
-  Variable psem: program -> interface -> semantics.
+  Variable sem: option program -> option semantics.
+  Variable psem: option program -> interface -> option semantics.
 End T.
 
 (* Intermediate *)
@@ -66,18 +97,11 @@ Module I <: Lang.
   Variable get_interface: program -> interface.
   Definition complete (p:program) := icomplete (get_interface p).
   Definition complete2 (p1 p2:program) := icomplete2 (get_interface p1) (get_interface p2).
-  Variable sem: program -> semantics.
-  Variable psem: program -> interface -> semantics.
+  Variable sem: option program -> option semantics.
+  Variable psem: option program -> interface -> option semantics.
 
   (* linking of two partial programs, returns a complete program *)
-  Variable link: program -> program -> program.
-  
-  Definition fully_defined (prg:program) :=
-    forall (ctx:program) (beh:program_behavior),
-      complete2 ctx prg ->
-      program_behaves (sem (link ctx prg)) beh ->
-      turn beh (get_interface prg) ->
-      not_wrong beh.
+  Variable link: program -> program -> option program.
 End I.
 
 (* Source *)
@@ -86,38 +110,39 @@ Module S <: Lang.
   Variable get_interface: program -> interface.
   Definition complete (p:program) := icomplete (get_interface p).
   Definition complete2 (p1 p2:program) := icomplete2 (get_interface p1) (get_interface p2).
-  Variable link: program -> program -> program.
-  Variable sem: program -> semantics.
-  Variable psem: program -> interface -> semantics.
+  Variable sem: option program -> option semantics.
+  Variable psem: option program -> interface -> option semantics.
 
-  Definition fully_defined (prg:program) :=
-    forall (ctx:program) (beh:program_behavior),
-      complete2 ctx prg ->
-      program_behaves (sem (link ctx prg)) beh ->
-      turn beh (get_interface prg) ->
-      not_wrong beh.
-        
-  Hypothesis definability :
-    forall beh (prg:program) psi,
-      icomplete2 (get_interface prg) psi ->
-      program_behaves (psem prg psi) beh ->
-      exists (ctx:program),
-        program_behaves (sem (link ctx prg)) beh.
+  Variable link: program -> program -> option program.
+  (* Variable link_prepost: *)
+  (*   forall (p1 p2 p:program), *)
+  (*     complete2 p1 p2 -> (link p1 p2 = Some p) /\ (get_interface p = (get_interface p1) ++ (get_interface p2)). *)
+
+  Definition fully_defined (psi:interface) (p:program) :=
+    forall (beh:program_behavior) (c:program),
+      get_interface c = psi ->
+      complete2 c p ->
+      behaves (sem (link c p)) beh ->
+      (turn beh (get_interface p) ->
+      not_wrong beh).
+
+  Hypothesis definability:
+    forall (beh:program_behavior) (psi:interface) (p:program),
+      icomplete2 psi (get_interface p) ->
+      behaves (psem (Some p) psi) beh ->
+      exists (c:program),
+        behaves (sem (link c p)) beh /\ get_interface c = psi.
 End S.
-
 
 
 (* This module takes a high language L1 and a low one L2 and produces
    a compiler from L1 to L2 and some properties *)
 Module Compiler (L1 L2: Lang).
   Variable compile : L1.program -> L2.program.
-
-  (* probably a corollary of partial compiler correctness *)
-  Hypothesis compiler_correctness :
-    forall beh (p:L1.program),
-      program_behaves (L2.sem (compile p)) beh ->
-      program_behaves (L1.sem p) beh.
-
+  Hypothesis compile_complete :
+    forall p1 p2,
+      L1.complete p1 -> compile p1 = p2 -> L2.complete p2.
+  
   Hypothesis compiler_interfaces:
   forall (p1:L1.program),
     L1.get_interface p1 = L2.get_interface (compile p1).
@@ -126,6 +151,12 @@ End Compiler.
 Module IT := Compiler I T.
 Module SI := Compiler S I.
 
+(* Hypothesis Tnotwrong : *)
+(*   forall b p, *)
+(*     program_behaves (T.sem p) b -> not_wrong b. *)
+(* Hypothesis Tpnotwrong : *)
+(*   forall b p psi, *)
+(*     program_behaves (T.psem p psi) b -> not_wrong b. *)
 
 (* 
    This property is different from the one we started from: there is
@@ -136,96 +167,89 @@ Module SI := Compiler S I.
    semantics by partializing a complete target program.
  *)
 
-
 Definition robust_compilation_static_compromise :=
   forall (c:I.program) (P:S.program) (beh:program_behavior),
-    icomplete2 (S.get_interface P) (I.get_interface c) ->
-    S.fully_defined P ->
-    program_behaves (T.sem (IT.compile (I.link c (SI.compile P)))) beh ->
-    exists C, program_behaves (S.sem (S.link C P)) beh.
+    icomplete2 (I.get_interface c) (S.get_interface P) ->
+    S.fully_defined (I.get_interface c) P ->
+    behaves (T.sem (map IT.compile (I.link c (SI.compile P)))) beh
+    ->
+    exists C, 
+      behaves (S.sem (S.link C P)) beh /\ S.complete2 C P.
 
-
+(* This definition is weaker than the above but has the advantage of
+   not mentioning the intermediate language *)
 Definition robust_compilation_static_compromise_corollary :=
   forall (Q P:S.program) (beh:program_behavior),
-    S.complete2 P Q ->
-    S.fully_defined P ->
-    program_behaves (T.sem (IT.compile (SI.compile (S.link Q P)))) beh ->
-    exists C, program_behaves (S.sem (S.link C P)) beh.
+    S.complete2 Q P ->
+    S.fully_defined (S.get_interface Q) P ->
+    let compile := compose IT.compile SI.compile in
+    behaves (T.sem (map compile (S.link Q P))) beh ->
+    exists C, behaves (S.sem (S.link C P)) beh /\ S.complete2 C P.
 
 (* This is too syntactic, it should be stated in terms of equivalent behaviors *)
 Hypothesis Sseparate_compilation:
   forall (P Q: S.program),
-    SI.compile (S.link P Q) = I.link (SI.compile P) (SI.compile Q).
+    map SI.compile (S.link Q P) = I.link (SI.compile Q) (SI.compile P).
 
 Corollary robust_compilation_corrolary :
   robust_compilation_static_compromise ->
   robust_compilation_static_compromise_corollary.
 Proof.
-  intros RC Q P b H1 H2 H3. specialize (RC (SI.compile Q) P b).
-  apply RC.
-  rewrite <- SI.compiler_interfaces with (p1:=Q).
-  auto.
-  auto.
-  rewrite Sseparate_compilation in H3.
-  auto.
+  intros RC Q P b Hcompl H1 H2 H3.
+  specialize (RC (SI.compile Q) P b).
+  rewrite <- SI.compiler_interfaces in RC.
+  unfold H2 in H3.
+  rewrite <- Sseparate_compilation in RC.
+  rewrite <- map_compose in H3.  
+  apply (RC Hcompl H1 H3).
 Qed.
 
 
 (* Extra ingredients needed for the proof. *)
 
-Hypothesis SIpcompiler_correctness :
-  forall beh (p:S.program) (psi:interface),
-    S.fully_defined p ->
-    program_behaves (I.psem (SI.compile p) psi) beh ->
-    program_behaves (S.psem p psi) beh.
-
-(* Takes a complete program and produces a partial one -- CH: potentially drop *)
-Variable Tpartialize: T.program -> interface -> T.program.
+(* takes a complete program and produces a partial one
+   This is an important ingredient for the simulation relation.
+   For MP the relation corresponds with this function actually.
+   For SFI the relation contains additional elements.
+ *)
+Variable Tpartialize: interface -> T.program -> T.program.
+(* Hypothesis partialize_post: *)
+(*   forall (p pp:T.program) psi, *)
+(*   Tpartialize psi p = pp -> *)
+(*   (T.get_interface p) = (T.get_interface pp)++psi. *)
 
 Hypothesis Tdecomposition:
   forall beh (c p:I.program),
-    program_behaves (T.sem (IT.compile (I.link c p))) beh ->
-    program_behaves (T.psem (Tpartialize (IT.compile (I.link c p)) (I.get_interface c)) (I.get_interface c)) beh.
+    let ip := map IT.compile (I.link c p) in
+    behaves (T.sem ip) beh
+    ->
+    behaves (T.psem (map (Tpartialize (I.get_interface c)) ip) (I.get_interface c)) beh.
+
+(* TODO IT.compile must be a refinement compiler *)
 
 Hypothesis ITspecial_pcompiler_correctness:
   forall beh (c p:I.program),
-    I.fully_defined p ->
-    program_behaves (T.psem (Tpartialize (IT.compile (I.link c p)) (I.get_interface c)) (I.get_interface c)) beh
-    ->
-    program_behaves (I.psem p (I.get_interface c)) beh.
+    (* I.fully_defined (I.get_interface c) p -> *)
+    let ip := I.link c p in
+    let tp := map (Tpartialize (I.get_interface c)) (map IT.compile ip) in
+    behaves (T.psem tp (I.get_interface c)) beh ->
+    behaves (I.psem (Some p) (I.get_interface c)) beh.
 
-Hypothesis Idecomposition:
-  forall beh (c p:I.program),
-    program_behaves (I.sem (I.link c p)) beh ->
-    program_behaves (I.psem p (I.get_interface c)) beh.
+(* exact cc preserves also UB *)
+Hypothesis SIpcompiler_correctness :
+  forall beh (p:S.program) (psi:interface),
+    behaves (I.psem (Some (SI.compile p)) psi) beh ->
+    behaves (S.psem (Some p) psi) beh.
 
-(* Lemma FD_preservation: *)
-(*   forall (P:S.program), *)
-(*     S.fully_defined P -> I.fully_defined (SI.compile P). *)
-(* Proof. *)
-(*   unfold I.fully_defined. *)
-(*   unfold S.fully_defined. *)
-(*   intros P FD c b Hcomplete H1 Hturn.  *)
-(*   apply Idecomposition in H1. *)
-(*   apply SIpcompiler_correctness in H1. *)
-(*   destruct (S.definability b P (I.get_interface c) H1) as [c2 H]. *)
-(*   unfold I.complete2 in Hcomplete. *)
-(*   rewrite <- SI.compiler_interfaces in Hcomplete. *)
-(*   unfold S.complete2 in FD. *)
-(*   apply (FD c2 b Hcomplete). *)
-(*   unfold S.fully_defined in FD. *)
-(*   specialize (FD (compile )) *)
-(*   rewrite <- Sseparate_compilation in H1. *)
-(*   apply SI.compiler_correctness in H1. *)
-(*   apply (FD c). *)
-  
 Theorem proof_rc_static : robust_compilation_static_compromise.
 Proof.
-  unfold robust_compilation_static_compromise.
-  intros c P b Hsplit HFD H.
-  apply Tdecomposition in H.
+  intros c P b Hcomplete SFD H.
+  apply (Tdecomposition b c (SI.compile P)) in H.
   apply ITspecial_pcompiler_correctness in H.
-  apply SIpcompiler_correctness in H.
-  apply S.definability in H.
-  auto. assumption. admit. (* probably corollary of SI[p?]compiler *)
-Admitted.
+  destruct (S.definability b (I.get_interface c) P Hcomplete) as [C [H1 Hinterfaces]].
+  apply (SIpcompiler_correctness b P (I.get_interface c)) in H.
+  assumption.
+  rewrite <- Hinterfaces in Hcomplete.
+  exists C.
+  auto.
+Qed.
